Some doodling with reflexive-transitive closure. Nearly proved big and small step equivalent for instructions.

Imps/Imp/Imp_SmallStep.v
@@ -38,6 +38,16 @@ match goal with
         assert (a1 = a2) by (eapply AEval_det; eauto); subst; clear H2
 end.
 
+Inductive rtc {A : Type} (R : A -> A -> Prop) : A -> A -> Prop :=
+    | rtc_step :
+        forall x y : A, R x y -> rtc R x y
+    | rtc_refl :
+        forall x : A, rtc R x x
+    | rtc_trans :
+        forall x y z : A, rtc R x y -> rtc R y z -> rtc R x z.
+
+Hint Constructors rtc.
+
 Inductive AEvals (s : State) : AExp -> AExp -> Prop :=
     | AEvals_step :
         forall a1 a2 : AExp,
@@ -81,25 +91,6 @@ Lemma AEvals_ABinOp :
     AEvals s (ABinOp f (AConst n1) (AConst n2)) (AConst (f n1 n2)).
 Proof. eauto. Qed.
 
-(*
-Lemma AEvals_ABinOp' :
-  forall (s : State) (f : nat -> nat -> nat) (a1 a1' a2 a2' : AExp),
-    AEvals s a1 a1' -> AEvals s a2 a2' ->
-      AEvals s (ABinOp f a1 a2) (ABinOp f a1' a2').
-Proof.
-  intros.
-  eapply AEvals_trans.
-    apply AEvals_ABinOp_L. eassumption.
-  eapply AEvals_trans.
-    apply AEvals_ABinOp_L. eassumption.
-      
-  induction 1. Focus 2. eauto. induction 1; eauto.
-    eapply AEvals_trans.
-      apply AEvals_step. apply AEval_ABinOp_L. eassumption.
-      apply AEvals_step.
-Admitted.
-*)
-
 Lemma aeval_AEvals :
   forall (s : State) (a : AExp) (n : nat),
     aeval s a = n -> AEvals s a (AConst n).
@@ -116,7 +107,7 @@ Proof.
 Qed.
 
 Lemma AEval_aevals :
-  forall (s : State) (a1 a2 : AExp),
+  forall {s : State} {a1 a2 : AExp},
     AEval s a1 a2 -> aeval s a1 = aeval s a2.
 Proof.
   induction 1; cbn; auto.
@@ -204,9 +195,6 @@ Admitted.
 *)
 
 (*
-Definition acompatible (a : AExp) (s1 s2 : State) : Prop :=
-  forall x : Loc, In x (loca a) -> s1 x = s2 x.
-
 Lemma AEval_acompatible_det :
   forall {s1 : State} {a a1 : AExp},
     AEval s1 a a1 -> forall {s2 : State},
@@ -230,7 +218,7 @@ Inductive BEval (s : State) : BExp -> BExp -> Prop :=
         forall (f : nat -> nat -> bool) (a1 a1' a2 : AExp),
           AEval s a1 a1' -> BEval s (BRelOp f a1 a2) (BRelOp f a1' a2)
     | BEval_BRelOp_R :
-        forall (f : nat -> nat -> bool) (n : nat) (a1 a2 a2' : AExp),
+        forall (f : nat -> nat -> bool) (n : nat) (a2 a2' : AExp),
           AEval s a2 a2' ->
             BEval s (BRelOp f (AConst n) a2) (BRelOp f (AConst n) a2')
     | BEval_BRelOp :
@@ -250,7 +238,7 @@ Inductive BEval (s : State) : BExp -> BExp -> Prop :=
             BEval s (BBinOp f (BConst b) e2) (BBinOp f (BConst b) e2')
     | BEval_BBinOp :
         forall (f : bool -> bool -> bool) (b1 b2 : bool),
-          BEval s (BBinOp f (BConst b1) (BConst b2)) (BConst (andb b1 b2)).
+          BEval s (BBinOp f (BConst b1) (BConst b2)) (BConst (f b1 b2)).
 
 Hint Constructors BEval.
 
@@ -268,23 +256,121 @@ Proof.
   end; eauto.
 Qed.
 
-(*
-Lemma BEval_beval :
+Ltac bdet := repeat
+match goal with
+    | H1 : BEval ?s ?e ?e1, H2 : BEval ?s ?e ?e2 |- _ =>
+        assert (e1 = e2) by (eapply BEval_det; eauto); subst; clear H2
+end.
+
+Lemma BEval_bevals :
   forall {s : State} {e1 e2 : BExp},
     BEval s e1 e2 -> beval s e1 = beval s e2.
 Proof.
-  induction 1; cbn.
-  rewrite ?(AEval_aeval H), ?IHBEval, ?IHBEval1, ?IHBEval2; auto.
+  Hint Resolve AEval_aevals.
+  induction 1; cbn;
+  rewrite ?(AEval_aevals H), ?IHBEval, ?IHBEval1, ?IHBEval2; auto.
 Qed.
 
-Lemma BEval_beval' :
-  forall {s : State} {e : BExp} {b : bool},
-    BEval s e (BConst b) -> beval s e = b.
+Definition BEvals (s : State) (e1 e2 : BExp) : Prop :=
+  rtc (BEval s) e1 e2.
+
+Hint Unfold BEvals.
+
+Lemma BEvals_BRelOp_L :
+  forall (s : State) (f : nat -> nat -> bool) (a1 a1' a2 : AExp),
+    AEvals s a1 a1' -> BEvals s (BRelOp f a1 a2) (BRelOp f a1' a2).
 Proof.
-  intros. change b with (beval s (BConst b)).
-  apply BEval_beval. assumption.
+  induction 1; eauto.
 Qed.
-*)
+
+Lemma BEvals_BRelOp_R :
+  forall (s : State) (f : nat -> nat -> bool) (n : nat) (a2 a2' : AExp),
+    AEvals s a2 a2' ->
+      BEvals s (BRelOp f (AConst n) a2) (BRelOp f (AConst n) a2').
+Proof.
+  induction 1; intros; eauto.
+Qed.
+
+Lemma BEvals_BRelOp :
+  forall (s : State) (f : nat -> nat -> bool) (n1 n2 : nat),
+    BEvals s (BRelOp f (AConst n1) (AConst n2)) (BConst (f n1 n2)).
+Proof. eauto. Qed.
+
+Lemma BEvals_Not_Step :
+  forall (s : State) (e e' : BExp),
+    BEvals s e e' -> BEvals s (Not e) (Not e').
+Proof.
+  induction 1; eauto.
+Qed.
+
+Lemma BEvals_Not :
+  forall (s : State) (b : bool),
+    BEvals s (Not (BConst b)) (BConst (negb b)).
+Proof. eauto. Qed.
+
+Lemma BEvals_BBinOp_L :
+  forall (s : State) (f : bool -> bool -> bool) (e1 e1' e2 : BExp),
+    BEvals s e1 e1' -> BEvals s (BBinOp f e1 e2) (BBinOp f e1' e2).
+Proof.
+  induction 1; eauto.
+Qed.
+
+Lemma BEvals_BBinOp_R :
+  forall (s : State) (f : bool -> bool -> bool) (b : bool) (e2 e2' : BExp),
+    BEvals s e2 e2' ->
+      BEvals s (BBinOp f (BConst b) e2) (BBinOp f (BConst b) e2').
+Proof.
+  induction 1; eauto.
+Qed.
+
+Lemma BEvals_BBinOp :
+  forall (s : State) (f : bool -> bool -> bool) (b1 b2 : bool),
+    BEvals s (BBinOp f (BConst b1) (BConst b2)) (BConst (f b1 b2)).
+Proof. eauto. Qed.
+
+Hint Resolve
+  BEvals_BRelOp_L BEvals_BRelOp_R BEvals_BRelOp
+  BEvals_Not_Step BEvals_Not
+  BEvals_BBinOp_L BEvals_BBinOp_R BEvals_BBinOp.
+
+Lemma beval_BEvals :
+  forall (s : State) (e : BExp) (b : bool),
+    beval s e = b -> BEvals s e (BConst b).
+Proof.
+  Hint Unfold BEvals.
+  induction e; cbn; intros.
+    inv H. auto.
+    inv H. eapply rtc_trans.
+      apply BEvals_BRelOp_L. apply aeval_AEvals. reflexivity.
+      eapply rtc_trans.
+        apply BEvals_BRelOp_R. apply aeval_AEvals. reflexivity.
+        apply BEvals_BRelOp.
+    inv H. eapply rtc_trans.
+      apply BEvals_Not_Step. apply IHe. reflexivity.
+      apply BEvals_Not.
+    inv H. eapply rtc_trans.
+      apply BEvals_BBinOp_L. apply IHe1. reflexivity.
+      eapply rtc_trans.
+        apply BEvals_BBinOp_R. apply IHe2. reflexivity.
+        apply BEvals_BBinOp.
+Qed.
+
+Lemma BEvals_bevals :
+  forall {s : State} {e1 e2 : BExp},
+    BEvals s e1 e2 -> beval s e1 = beval s e2.
+Proof.
+  induction 1; cbn; intros.
+    apply BEval_bevals. assumption.
+    reflexivity.
+    rewrite IHrtc1, IHrtc2. reflexivity.
+Qed.
+
+Lemma BEvals_beval :
+  forall (s : State) (e : BExp) (b : bool),
+    BEvals s e (BConst b) -> beval s e = b.
+Proof.
+  intros. apply BEvals_bevals in H. cbn in H. assumption.
+Qed.
 
 (*
 Lemma BEval_bcompatible_det :
@@ -306,130 +392,271 @@ Proof.
 Qed.
 *)
 
-Inductive CEval : Com * State -> Com * State + State -> Prop :=
-    | EvalSkip :
-        forall s : State, CEval (Skip, s) (inr s)
-    | EvalAsgnStep :
+Lemma Imp_BigStep_SmallStep_logic :
+  forall (s : State) (e : BExp) (b : bool),
+    Imp_BigStep.BEval e s b <-> BEvals s e (BConst b).
+Proof.
+  split; intro.
+    apply Imp_BigStep.BEval_beval in H. apply beval_BEvals. assumption.
+    apply BEvals_beval in H. apply Imp_BigStep.beval_BEval. assumption.
+Qed.
+
+Inductive CEval : Com * State -> Com * State -> Prop :=
+    | CEval_Asgn_Step :
         forall (s : State) (a a' : AExp) (x : Loc),
-          AEval s a a' -> CEval (Asgn x a, s) (inl (Asgn x a', s))
-    | EvalAsgnVal :
+          AEval s a a' -> CEval (Asgn x a, s) (Asgn x a', s)
+    | CEval_Asgn_Val :
         forall (s : State) (n : nat) (x : Loc),
-          CEval (Asgn x (AConst n), s) (inr (changeState s x n))
-    | EvalSeqL :
+          CEval (Asgn x (AConst n), s) (Skip, changeState s x n)
+    | CEval_Seq_L :
         forall (c1 c1' c2 : Com) (s s' : State),
-          CEval (c1, s) (inl (c1', s')) ->
-            CEval (Seq c1 c2, s) (inl (Seq c1' c2, s'))
-    | EvalSeqR :
-        forall (c1 c2 : Com) (s s' : State),
-          CEval (c1, s) (inr s') -> CEval (Seq c1 c2, s) (inl (c2, s'))
-    | EvalIfCond :
+          CEval (c1, s) (c1', s') ->
+            CEval (Seq c1 c2, s) (Seq c1' c2, s')
+    | CEval_Seq_R :
+        forall (c : Com) (s : State),
+          CEval (Seq Skip c, s) (c, s)
+    | CEval_If_Step :
         forall (b b' : BExp) (c1 c2 : Com) (s : State),
-          BEval s b b' -> CEval (If b c1 c2, s) (inl (If b' c1 c2, s))
-    | EvalIfTrue :
+          BEval s b b' -> CEval (If b c1 c2, s) (If b' c1 c2, s)
+    | CEval_If_True :
         forall (s : State) (c1 c2 : Com),
-          CEval (If (BConst true) c1 c2, s) (inl (c1, s))
-    | EvalIfFalse :
+          CEval (If (BConst true) c1 c2, s) (c1, s)
+    | CEval_If_False :
         forall (s : State) (c1 c2 : Com),
-          CEval (If (BConst false) c1 c2, s) (inl (c2, s))
-    | EvalWhile :
+          CEval (If (BConst false) c1 c2, s) (c2, s)
+    | CEval_While :
         forall (b : BExp) (c : Com) (s : State),
-          CEval (While b c, s) (inl (If b (Seq c (While b c)) Skip, s)).
+          CEval (While b c, s) (If b (Seq c (While b c)) Skip, s).
 
 Hint Constructors CEval.
 
 Lemma CEval_det :
-  forall {cs : Com * State} {cs1 : Com * State + State},
-    CEval cs cs1 -> forall {cs2 : Com * State + State},
+  forall {cs cs1 : Com * State},
+    CEval cs cs1 -> forall {cs2 : Com * State},
       CEval cs cs2 -> cs1 = cs2.
 Proof.
-  Hint Resolve AEval_det BEval_det.
   induction 1; intros; repeat
   match goal with
+      | H : AEval _ ?x _ |- _ => tryif is_var x then fail else inv H
+      | H : BEval _ ?x _ |- _ => tryif is_var x then fail else inv H
+      | H : CEval (?x, _) _ |- _ => tryif is_var x then fail else inv H
       | IH : forall _, CEval _ _ -> _, H : CEval _ _ |- _ =>
           let H' := fresh "H" in
             pose (H' := IH _ H); inv H'; clear H
-      | |- ?f _ = ?f _ => f_equal; eauto
-      | |- ?f _ _ = ?f _ _ => f_equal; eauto
-      | |- ?f _ _ _ = ?f _ _ _ => f_equal; eauto
-      | H : AEval _ (?f _) _ |- _ => inv H
-      | H : BEval _ (?f _) _ |- _ => inv H
-      | H : CEval (?f _ _) _ |- _ => inv H
+      | _ => adet; bdet; auto
   end.
 Qed.
 
-(*Hint Immediate aeval_AEval beval_BEval.*)
+Ltac cdet := repeat
+match goal with
+    | H1 : CEval ?cs ?cs1, H2 : CEval ?cs ?cs2 |- _ =>
+        assert (cs1 = cs2) by (eapply CEval_det; eauto); subst; clear H2
+end.
 
-Inductive CEval' : Com * State -> State -> Prop :=
-    | CEval'_step :
-        forall (cs : Com * State) (s : State),
-          CEval cs (inr s) -> CEval' cs s
-    | CEval'_more :
-        forall (cs1 cs2 : Com * State) (s : State),
-          CEval cs1 (inl cs2) -> CEval' cs2 s -> CEval' cs1 s.
+Definition CEvals (cs1 cs2 : Com * State) : Prop :=
+  rtc CEval cs1 cs2.
 
-Hint Constructors CEval'.
+Hint Unfold CEvals.
 
-(*
-Lemma ceval_CEval' :
-  forall (n : nat) (c : Com) (s1 s2 : State),
-    ceval n c s1 = Some s2 -> CEval' (c, s1) s2.
+Lemma CEval_cevals :
+  forall {cs1 cs2 : Com * State},
+    CEval cs1 cs2 -> forall {n : nat} {s : State},
+      ceval n (fst cs2) (snd cs2) = Some s ->
+      ceval (S n) (fst cs1) (snd cs2) = Some s.
 Proof.
-  intros n c s1.
-  functional induction ceval n c s1; intros; inv H; eauto.
-    constructor. Print CEval.
+  induction 1; cbn.
+    destruct n; cbn; intros.
+      inv H0.
+      inv H0. do 2 f_equal. apply AEval_aevals. assumption.
+    destruct n0; cbn; intros; auto.
+      inv H.
+      inv H. compute. f_equal. admit.
+    all: destruct n as [| n']; cbn in *; intros; eauto.
+      Focus 2. inv H0.
+      Focus 2. apply BEval_bevals in H. rewrite H. destruct (beval s b').
+        destruct c1; inv H0.
+Restart.
+  intros. revert cs1 H s H0.
+  functional induction ceval n (fst cs2) (snd cs2); intros; try congruence.
+    inv H0.
+Admitted.
+
+Lemma CEvals_Asgn_Step :
+  forall (s : State) (a a' : AExp) (x : Loc),
+    AEvals s a a' -> CEvals (Asgn x a, s) (Asgn x a', s).
+Proof.
+  induction 1; eauto.
 Qed.
 
-Lemma ceval_plus :
-  forall (n k : nat) (c : Com) (s1 s2 : State),
-    ceval n c s1 = Some s2 -> ceval (n + k) c s1 = Some s2.
+Lemma CEvals_Asgn_Val :
+  forall (s : State) (n : nat) (x : Loc),
+    CEvals (Asgn x (AConst n), s) (Skip, changeState s x n).
+Proof. eauto. Qed.
+
+Lemma CEvals_Seq_L :
+  forall (c1 c1' c2 : Com) (s s' : State),
+    CEvals (c1, s) (c1', s') ->
+      CEvals (Seq c1 c2, s) (Seq c1' c2, s').
 Proof.
-  induction n as [| n']; cbn; intros.
+Admitted.
+
+Lemma CEvals_Seq_R :
+  forall (c : Com) (s : State),
+    CEvals (Seq Skip c, s) (c, s).
+Proof. eauto. Qed.
+
+Lemma CEvals_If_Step :
+  forall (b b' : BExp) (c1 c2 : Com) (s : State),
+    BEvals s b b' -> CEvals (If b c1 c2, s) (If b' c1 c2, s).
+Proof.
+  induction 1; eauto.
+Qed.
+
+Lemma CEvals_If_True :
+  forall (s : State) (c1 c2 : Com),
+    CEvals (If (BConst true) c1 c2, s) (c1, s).
+Proof. eauto. Qed.
+
+Lemma CEvals_If_False :
+  forall (s : State) (c1 c2 : Com),
+    CEvals (If (BConst false) c1 c2, s) (c2, s).
+Proof. eauto. Qed.
+
+Lemma CEvals_While :
+  forall (b : BExp) (c : Com) (s : State),
+    CEvals (While b c, s) (If b (Seq c (While b c)) Skip, s).
+Proof. eauto. Qed.
+
+Lemma ceval_CEvals :
+  forall (n : nat) (c : Com) (s s' : State),
+    ceval n c s = Some s' -> CEvals (c, s) (Skip, s').
+Proof.
+  intros n c s. functional induction ceval n c s; cbn; intros.
     inv H.
-    destruct c; auto.
-      destruct (ceval n' c1 s1) eqn: Heq.
-        erewrite IHn'; eauto.
-        inv H.
-      destruct (beval b s1) eqn: Hb; eauto.
-      destruct (beval b s1) eqn: Hb; eauto.
-        destruct (ceval n' c s1) eqn: Heq.
-          erewrite IHn'; eauto.
-          inv H.
+    inv H. auto.
+    inv H. eapply rtc_trans.
+      apply CEvals_Asgn_Step. apply aeval_AEvals. reflexivity.
+      eauto.
+    inv H.
+    eapply rtc_trans.
+      apply CEvals_Seq_L. eauto.
+      eapply rtc_trans.
+        apply CEvals_Seq_R. apply IHo0. assumption.
+    eapply rtc_trans.
+      apply CEvals_If_Step. apply beval_BEvals. eassumption.
+      eapply rtc_trans.
+        apply CEvals_If_True.
+        apply IHo. assumption.
+    eapply rtc_trans.
+      apply CEvals_If_Step. apply beval_BEvals. eassumption.
+      eapply rtc_trans.
+        apply CEvals_If_False.
+        apply IHo. assumption.
+    inv H.
+    eapply rtc_trans.
+      apply CEvals_While. eapply rtc_trans.
+        eapply CEvals_If_Step. apply beval_BEvals. eassumption.
+        eapply rtc_trans.
+          apply CEvals_If_True.
+          eapply rtc_trans.
+            apply CEvals_Seq_L. eauto.
+            eapply rtc_trans.
+              apply CEvals_Seq_R.
+              apply IHo0. assumption.
+    eapply rtc_trans.
+      apply CEvals_While. eapply rtc_trans.
+        eapply CEvals_If_Step. apply beval_BEvals. eassumption.
+        eapply rtc_trans.
+          apply CEvals_If_False.
+          inv H. auto.
 Qed.
 
-Lemma CEval_ceval :
-  forall (c : Com) (s1 s2 : State),
-    CEval c s1 s2 -> exists n : nat, ceval n c s1 = Some s2.
+Inductive rtc' {A : Type} (R : A -> A -> Prop) : A -> A -> Prop :=
+    | rtc'_refl :
+        forall x : A, rtc' R x x
+    | rtc'_steptrans :
+        forall x y z : A, R x y -> rtc' R y z -> rtc' R x z.
+
+Hint Constructors rtc'.
+
+Definition CEvals' (cs1 cs2 : Com * State) : Prop :=
+  rtc' CEval cs1 cs2.
+
+Hint Unfold CEvals'.
+
+Lemma rtc'_trans :
+  forall {A : Type} {R : A -> A -> Prop} {x y z : A},
+    rtc' R x y -> rtc' R y z -> rtc' R x z.
 Proof.
-  induction 1.
-    exists 1. cbn. reflexivity.
-    exists 1. cbn. do 2 f_equal. apply AEval_aeval. assumption.
-    destruct IHCEval1 as [n1 IH1], IHCEval2 as [n2 IH2].
-      exists (S (n1 + n2)). (* Should be S (max n1 n2) *)
-      cbn. rewrite (ceval_plus n1 n2 _ _ _ IH1), plus_comm.
-        apply ceval_plus. assumption.
-    destruct IHCEval as [n IH]. exists (S n). cbn.
-      apply BEval_beval in H. rewrite H. assumption.
-    destruct IHCEval as [n IH]. exists (S n). cbn.
-      apply BEval_beval in H. rewrite H. assumption.
-    exists 1. cbn. apply BEval_beval in H. rewrite H. reflexivity.
-    destruct IHCEval1 as [n1 IH1], IHCEval2 as [n2 IH2].
-      exists (S (n1 + n2)). cbn. (* Should be S (max n1 n2) *)
-      apply BEval_beval in H. rewrite H.
-      rewrite (ceval_plus _ _ _ _ _ IH1), plus_comm.
-      apply ceval_plus. assumption.
+  intros until 1. revert z.
+  induction H; intros.
+    assumption.
+    eauto.
+Qed.
+
+Lemma CEvals_CEvals' :
+  forall cs1 cs2 : Com * State,
+    CEvals cs1 cs2 -> CEvals' cs1 cs2.
+Proof.
+  unfold CEvals; unfold CEvals'.
+  induction 1; eauto.
+  eapply rtc'_trans; eauto.
+Qed.
+
+Lemma CEvals'_ceval :
+  forall (c : Com) (s1 s2 : State),
+    CEvals' (c, s1) (Skip, s2) -> exists n : nat,
+      ceval n c s1 = Some s2.
+Proof.
+  intros c s1 s2 H.
+  remember (c, s1) as cs1.
+  remember (Skip, s2) as cs2.
+  revert c s1 s2 Heqcs1 Heqcs2.
+  induction H; intros.
+    inv Heqcs1. inv Heqcs2. exists 1. cbn. reflexivity.
+    inv Heqcs1. destruct y.
+      destruct  (IHrtc' _ _ _ eq_refl eq_refl) as [n IH].
+      exists (S n). cbn. inv H. cbn in *.
+Admitted.
+
+Lemma CEvals_ceval :
+  forall (c : Com) (s1 s2 : State),
+    CEvals (c, s1) (Skip, s2) -> exists n : nat,
+      ceval n c s1 = Some s2.
+Proof.
+  intros c s1 s2 H.
+  remember (c, s1) as cs1.
+  remember (Skip, s2) as cs2.
+  revert c s1 s2 Heqcs1 Heqcs2.
+  induction H; intros.
+    inv Heqcs1. inv H.
+      exists 1. cbn. reflexivity.
+      1-3: exists 2; cbn; reflexivity.
+    inv Heqcs1. inv Heqcs2. exists 1. cbn. reflexivity.
+    inv Heqcs1. inv H.
+Admitted.
+
+Lemma Imp_BigStep_SmallStep_Com :
+  forall (c : Com) (s1 s2 : State),
+    Imp_BigStep.CEval c s1 s2 <-> CEvals (c, s1) (Skip, s2).
+Proof.
+  split; intro.
+    apply Imp_BigStep.CEval_ceval in H. destruct H as [n H].
+      eapply ceval_CEvals. eassumption.
+    apply CEvals_ceval in H. destruct H as [n H].
+      apply Imp_BigStep.ceval_CEval with n. assumption.
 Qed.
 
 Lemma while_true_do_skip :
   forall s1 s2 : State,
-    ~ CEval (While BTrue Skip) s1 s2.
+    ~ CEval (While (BConst true) Skip, s1) (Skip, s2).
 Proof.
   intros s1 s2 H.
-  remember (While BTrue Skip) as w. revert Heqw.
-  induction H; intros; inv Heqw.
-    inv H.
-    apply IHCEval2. reflexivity.
+  remember (While (BConst true) Skip, s1) as cs1.
+  remember (Skip, s2) as cs2.
+  revert s1 s2 Heqcs1 Heqcs2.
+  induction H; intros; inv Heqcs1; inv Heqcs2.
 Qed.
-
 
 (*
 Lemma CEval_not_In_locw_eq :
@@ -505,182 +732,4 @@ Proof.
           eapply IHCEval2; eauto. intros. apply in_app_or in H5. inv H5.
 *)
 Abort.
-
-(* Program equivalence. *)
-
-Definition equivalent (c1 c2 : Com) : Prop :=
-  forall s1 s2 : State,
-    CEval c1 s1 s2 <-> CEval c2 s1 s2.
-
-Notation "c1 ~ c2" := (equivalent c1 c2) (at level 50).
-
-Example equivalent_ex1 :
-  forall (b : BExp) (c : Com),
-    While b c ~ If b (Seq c (While b c)) Skip.
-Proof.
-  unfold equivalent. split; intros.
-    remember (While b c) as w. revert b c Heqw.
-      induction H; intros; inv Heqw; eauto.
-    inv H; inv H6; eauto.
-Defined.
-
-(* TODO: for loop *)
-
-Inductive Context : Type :=
-    | CContext : Context
-    | CSeqL : Context -> Com -> Context
-    | CSeqR : Com -> Context -> Context
-    | CIfL : BExp -> Context -> Com -> Context
-    | CIfR : BExp -> Com -> Context -> Context
-    | CWhile : BExp -> Context -> Context.
-
-Fixpoint put (G : Context) (c : Com) : Com :=
-match G with
-    | CContext => c
-    | CSeqL G' c' => Seq (put G' c) c'
-    | CSeqR c' G' => Seq c' (put G' c)
-    | CIfL b G' c' => If b (put G' c) c'
-    | CIfR b c' G' => If b c' (put G' c)
-    | CWhile b G' => While b (put G' c)
-end.
-
-Lemma equivalent_in_Context :
-  forall c1 c2 : Com,
-    c1 ~ c2 -> forall G : Context, put G c1 ~ put G c2.
-Proof.
-  intros c1 c2 H G. revert c1 c2 H.
-  induction G; cbn; intros.
-    assumption.
-    all: unfold equivalent in *; split; intros.
-      inv H0. econstructor.
-        rewrite IHG; eauto. firstorder.
-        assumption.
-      inv H0. econstructor; rewrite 1?IHG; eauto.
-      inv H0. econstructor; rewrite 1?IHG; eauto. firstorder.
-      inv H0. econstructor; rewrite 1?IHG; eauto.
-      inv H0.
-        econstructor; rewrite 1?IHG; eauto.
-        apply EvalIfTrue; eauto. rewrite IHG; eauto. firstorder.
-      inv H0.
-        econstructor; rewrite 1?IHG; eauto.
-        apply EvalIfTrue; eauto. rewrite IHG; eauto.
-      inv H0.
-        econstructor; rewrite 1?IHG; eauto. firstorder.
-        apply EvalIfTrue; eauto.
-      inv H0.
-        econstructor; rewrite 1?IHG; eauto.
-        firstorder.
-      remember (While b (put G c1)) as w. revert Heqw.
-      induction H0; intro; inv Heqw.
-        eauto.
-        econstructor; eauto. rewrite IHG; eauto. firstorder.
-      remember (While b (put G c2)) as w. revert Heqw.
-      induction H0; intro; inv Heqw.
-        eauto.
-        econstructor; eauto. rewrite IHG; eauto.
-Restart.
-  intros c1 c2 H G. revert c1 c2 H.
-  induction G; cbn; intros; eauto;
-  unfold equivalent in *; split; intros;
-  match goal with
-      | H : CEval ?c _ _ |- _ =>
-          let c' := fresh "c" in
-          let Heqc' := fresh "Heq" c' in
-            remember c as c'; revert Heqc';
-            induction H; intros; inv Heqc'
-  end; eauto.
-    5-6: apply EvalIfTrue; rewrite 1?IHG; eauto; firstorder.
-    all: econstructor; rewrite 1?IHG; eauto; firstorder.
-Qed.
-
-(** [equivalent] is a congruence *)
-
-Lemma equivalent_Seq_l :
-  forall c c1 c2 : Com,
-    c1 ~ c2 -> Seq c1 c ~ Seq c2 c.
-Proof.
-  unfold equivalent. split; intros.
-    inv H0. econstructor.
-      rewrite <- H. eassumption.
-      assumption.
-    inv H0. econstructor.
-      rewrite H. eassumption.
-      assumption.
-Qed.
-
-Lemma equivalent_Seq_r :
-  forall c c1 c2 : Com,
-    c1 ~ c2 -> Seq c c1 ~ Seq c c2.
-Proof.
-  unfold equivalent. split; intros.
-    inv H0. econstructor.
-      eassumption.
-      rewrite <- H. eassumption.
-    inv H0. econstructor.
-      eassumption.
-      rewrite H. eassumption.
-Qed.
-
-Lemma equivalent_If_l :
-  forall (b : BExp) (c c1 c2 : Com),
-    c1 ~ c2 -> If b c1 c ~ If b c2 c.
-Proof.
-  unfold equivalent. split; intros.
-    inv H0.
-      constructor; assumption.
-      apply EvalIfTrue.
-        assumption.
-        rewrite <- H. assumption.
-    inv H0.
-      constructor; assumption.
-      apply EvalIfTrue.
-        assumption.
-        rewrite H. assumption.
-Qed.
-
-Lemma equivalent_If_r :
-  forall (b : BExp) (c c1 c2 : Com),
-    c1 ~ c2 -> If b c c1 ~ If b c c2.
-Proof.
-  unfold equivalent. split; intros.
-    inv H0.
-      constructor.
-        assumption.
-        rewrite <- H. assumption.
-      apply EvalIfTrue; assumption.
-    inv H0.
-      constructor.
-        assumption.
-        rewrite H. assumption.
-      apply EvalIfTrue; assumption.
-Qed.
-
-Lemma equivalent_While :
-  forall (b : BExp) (c c1 c2 : Com),
-    c1 ~ c2 -> While b c1 ~ While b c2.
-Proof.
-  unfold equivalent. split; intros.
-    remember (While b c1) as w. revert Heqw. induction H0; intro; inv Heqw.
-      constructor. assumption.
-      eapply EvalWhileTrue.
-        assumption.
-        rewrite <- H. eassumption.
-        apply IHCEval2. reflexivity.
-    remember (While b c2) as w. revert Heqw. induction H0; intro; inv Heqw.
-      constructor. assumption.
-      eapply EvalWhileTrue.
-        assumption.
-        rewrite H. eassumption.
-        apply IHCEval2. reflexivity.
-Qed.
-
-(** * Observational equivalence *)
-
-Definition Observation (A : Type) : Type := Com -> A.
-
-Definition oequiv {A : Type} (c1 c2 : Com) : Prop :=
-  forall (G : Context) (f : Observation A),
-    f (put G c1) = f (put G c2).
-*)
-
 *)
